picker

Examples.v
@@ -1,13 +1,75 @@
-Require Import Process Refinement.
+Require Import Process Refinement List Eqdep_dec.
 
 
-Ltac normalize := solve [ eapply normBasic; repeat (constructor; intros) ].
+Ltac normalize := repeat (solve [ apply normProcD | eapply normBasic; repeat (constructor; intros) ]
+                       || eapply normParallel).
+
+Ltac inverter H := let H' := fresh "H'" in
+                   generalize H; intro H'; apply (f_equal (@Chans _)) in H'; simpl in H'; subst;
+                   apply (f_equal (@Code _)) in H; simpl in H; subst.
+
+Definition channelOf {chs} (p : proc0 chs) :=
+  match p with
+  | NSend ch _ _ => ch
+  | NRecv ch _ => ch
+  | NDone => ""
+  end.
+
+Inductive simplified {chs} (ch : string) : Type :=
+| SSend (v : chs ch) (k : proc0 chs)
+| SRecv (k : chs ch -> proc0 chs)
+| SDone.
+
+Definition simplify {chs} (p : proc0 chs) : simplified (channelOf p) :=
+  match p with
+  | NSend _ v k => SSend _ v k
+  | NRecv _ k => SRecv _ k
+  | NDone => SDone _
+  end.
+
+Require Import Eqdep_dec.
+
+Ltac inverter2 H := let H' := fresh "H'" in generalize H; intro H';
+                    apply (f_equal (@channelOf _)) in H'; simpl in H'; subst;
+                    apply (f_equal (fun x => existT simplified (channelOf x) (simplify x))) in H;
+                    simpl in H; apply (inj_pair2_eq_dec _ string_dec) in H; inv H.
+
+Ltac oneStep0 :=
+  match goal with
+  | _ => discriminate
+  | [ H : _ :: _ = _ :: _ |- _ ] => 
+    inversion H; clear H; intros;
+    repeat match goal with
+                                  | [ x : _ |- _ ] => subst x
+                                  | [ H : existT _ _ _ = existT _ _ _ |- _ ] =>
+                                    apply (inj_pair2_eq_dec _ string_dec) in H; subst
+           end
+  | [ H : pick1 ?ls _ _ |- _ ] => remember ls; inv H
+
+  | [ H : Build_proc _ _ _ = Build_proc _ _ _ |- _ ] => inverter H
+  | [ H : NSend _ _ _ _ = NSend _ _ _ _ |- _ ] => inverter2 H
+  | [ H : NRecv _ _ _ = NRecv _ _ _ |- _ ] => inverter2 H
+  end.
+
+Ltac oneStep' := simpl; intros; repeat oneStep0.
 
 Ltac oneStep :=
-  apply oneStep; simpl; intros;
-  repeat match goal with
-         | [ H : pick1 _ _ _ |- _ ] => inv H
-         end.
+  apply oneStep; oneStep'.
+
+Ltac picker' ls toHere k :=
+  match ls with
+  | _ :: ?ls' =>
+    k ltac:(toHere; apply Fst1)
+    || picker' ls' ltac:(toHere; apply More1) k
+  end.
+
+Ltac picker :=
+  match goal with
+  | [ |- exists P k ps', pick1 ?ls _ _ /\ P _ /\ refines _ _ ] =>
+    picker' ls idtac ltac:(fun tac => do 4 esplit; [ tac | split; [ simpl; tauto | ] ])
+  end.
+
+Ltac refines := eapply refines_normalize; [ normalize | normalize | oneStep; try picker ].
 
 Module DoneDone.
   Definition chs : channels := fun _ => nat.
@@ -18,9 +80,33 @@ Module DoneDone.
 
   Theorem pr1_pr2 : refines pr1 pr2.
   Proof.
-    eapply refines_normalize.
-    normalize.
-    normalize.
-    oneStep.
+    refines.
   Qed.
 End DoneDone.
+
+Module DoneSend.
+  Definition chs : channels := fun _ => nat.
+
+  Definition pr1 : process chs := Done.
+
+  Definition pr2 : process chs := #!chs["X", 0], Done.
+
+  Theorem pr1_pr2 : refines pr1 pr2.
+  Proof.
+    refines.
+  Qed.
+End DoneSend.
+
+Module SendSend.
+  Definition chs : channels := fun _ => nat.
+
+  Definition pr1 : process chs := #!chs["X", 0], Done.
+
+  Definition pr2 : process chs := #!chs["X", 0], Done.
+
+  Theorem pr1_pr2 : refines pr1 pr2.
+  Proof.
+    refines.
+    refines.
+  Qed.
+End SendSend.
